Exp.thy
@@ -2,63 +2,132 @@ theory Exp
   imports Definitions
 begin
 
+section \<open>Semantics of Expressions\<close>
+
+text \<open>This section presents the big-step semantics of expressions.\<close>
+
 inductive exp_sem :: 
-  "gamma * heap * reborrow * exp \<Rightarrow> heap * reborrow * val \<Rightarrow> bool" (infix "\<Down>" 65)
+  "gamma * heap * exp \<Rightarrow> heap * val \<Rightarrow> bool" (infix "\<Down>" 65)
 where
-  Const: "(\<Gamma>, H, R, Const v) \<Down> (H, R, v)" |
-  Var: "the (\<Gamma> x) = v \<Longrightarrow> (\<Gamma>, H, R, Var x) \<Down> (H, R, v)" |
-  Box: "\<lbrakk>(\<Gamma>, H, R, e) \<Down> (H', R', v); fresh p H'; fresh_tag t R'\<rbrakk> 
-        \<Longrightarrow> (\<Gamma>, H, R, Box e) \<Down> (H'(p \<mapsto> v), R'(p \<mapsto> [t]), Reference p t)" |
-  Reborrow: "\<lbrakk>(\<Gamma>, H, R, e) \<Down> (H', R', Reference p t); writable p t R'; fresh_tag t' R'\<rbrakk>
-             \<Longrightarrow> (\<Gamma>, H, R, Reborrow e) \<Down> (H', R'(p \<mapsto> kill t (the (R' p)) @ [t']), Reference p t')" |
-  Deref: "\<lbrakk>(\<Gamma>, H, R, e) \<Down> (H', R', Reference p t); readable p t R'; v = the (H' p)\<rbrakk>
-          \<Longrightarrow> (\<Gamma>, H, R, Deref e) \<Down> (H', R'(p \<mapsto> kill t (the (R' p))), v)" |
-  Plus: "\<lbrakk>(\<Gamma>, H, R, e1) \<Down> (H', R', VInt i1); (\<Gamma>, H', R', e2) \<Down> (H'', R'', VInt i2)\<rbrakk>
-         \<Longrightarrow> (\<Gamma>, H, R, Plus e1 e2) \<Down> (H'', R'', VInt (i1 + i2))" |
-  Less: "\<lbrakk>(\<Gamma>, H, R, e1) \<Down> (H', R', VInt i1); (\<Gamma>, H', R', e2) \<Down> (H'', R'', VInt i2)\<rbrakk>
-         \<Longrightarrow> (\<Gamma>, H, R, Less e1 e2) \<Down> (H'', R'', VBool (i1 < i2))" |
-  Not: "(\<Gamma>, H, R, e) \<Down> (H', R', VBool b) \<Longrightarrow> (\<Gamma>, H, R, Not e) \<Down> (H', R', VBool (\<not>b))" |
-  And: "\<lbrakk>(\<Gamma>, H, R, e1) \<Down> (H', R', VBool b1); (\<Gamma>, H', R', e2) \<Down> (H'', R'', VBool b2)\<rbrakk>
-         \<Longrightarrow> (\<Gamma>, H, R, And e1 e2) \<Down> (H'', R'', VBool (b1 \<and> b2))"
-
-lemmas exp_sem_cases = exp_sem.cases[split_format(complete)]
-lemmas exp_sem_induct = exp_sem.induct[split_format(complete)]
-declare exp_sem.intros[simp]
-
-inductive_cases ConstE[elim!]: "(\<Gamma>, H, R, Const v) \<Down> v'"
-thm ConstE
-inductive_cases VarE[elim!]: "(\<Gamma>, H, R, Var x) \<Down> v"
-thm VarE
-inductive_cases BoxE[elim!]: "(\<Gamma>, H, R, Box e) \<Down> v"
-thm BoxE
-inductive_cases ReborrowE[elim!]: "(\<Gamma>, H, R, Reborrow e) \<Down> v"
-thm ReborrowE
-inductive_cases DerefE[elim!]: "(\<Gamma>, H, R, Deref e) \<Down> v"
-thm DerefE
+  Const: "(\<Gamma>, H, Const v) \<Down> (H, v)" |
+  Var: "the (\<Gamma> x) = v \<Longrightarrow> (\<Gamma>, H, Var x) \<Down> (H, v)" |
+  Box: "\<lbrakk>(\<Gamma>, H, e) \<Down> (H', v); p = length H'; t = fresh_tag H'\<rbrakk> 
+        \<Longrightarrow> (\<Gamma>, H, Box e) \<Down> (H' @ [(v, [t])], Reference p t)" |
+  Reborrow: "\<lbrakk>(\<Gamma>, H, e) \<Down> (H', Reference p t); writable p t H'; (v, ts) = H' ! p; t' = fresh_tag H'\<rbrakk>
+             \<Longrightarrow> (\<Gamma>, H, Reborrow e) \<Down> (H'[p := (v, (kill t ts) @ [t'])], Reference p t')" |
+  Deref: "\<lbrakk>(\<Gamma>, H, e) \<Down> (H', Reference p t); readable p t H'; (v, ts) = H' ! p\<rbrakk>
+          \<Longrightarrow> (\<Gamma>, H, Deref e) \<Down> (H'[p := (v, kill t ts)], v)" |
+  Plus: "\<lbrakk>(\<Gamma>, H, e1) \<Down> (H', VInt i1); (\<Gamma>, H', e2) \<Down> (H'', VInt i2)\<rbrakk>
+         \<Longrightarrow> (\<Gamma>, H, Plus e1 e2) \<Down> (H'', VInt (i1 + i2))" |
+  Less: "\<lbrakk>(\<Gamma>, H, e1) \<Down> (H', VInt i1); (\<Gamma>, H', e2) \<Down> (H'', VInt i2)\<rbrakk>
+         \<Longrightarrow> (\<Gamma>, H, Less e1 e2) \<Down> (H'', VBool (i1 < i2))" |
+  Not: "(\<Gamma>, H, e) \<Down> (H', VBool b) \<Longrightarrow> (\<Gamma>, H, Not e) \<Down> (H', VBool (\<not>b))" |
+  And: "\<lbrakk>(\<Gamma>, H, e1) \<Down> (H', VBool b1); (\<Gamma>, H', e2) \<Down> (H'', VBool b2)\<rbrakk>
+         \<Longrightarrow> (\<Gamma>, H, And e1 e2) \<Down> (H'', VBool (b1 \<and> b2))"
 
 text \<open>
-  We have nice derivation trees as shown in Figure \ref{fig:exp}.
-  Note that the validity of reference is not checked in the current
-  REBORROW and DEREF rules.
-\begin{figure}[h]
-  \centering
+We present the intuition behind the selected rules.
+First, {\sc{Box}} rule allocates a new slot at the end of heap,
+returning a reference pointing to the slot with a fresh tag.
+
 \begin{framed}
-  @{thm[mode=Rule] Var} \sc{Var}\\
-  @{thm[mode=Rule] Box} \sc{Box} \\
-  @{thm[mode=Rule] Reborrow} \sc{Reborrow} \\
-  @{thm[mode=Rule] Deref} \sc{Deref}
+\centering
+@{thm[mode=Rule] Box} \sc{Box}
 \end{framed}
-  \caption{Selected derivation rules for expressions}
-  \label{fig:exp}
-\end{figure}
+
+Next, {\sc{Deref}} rule allows us to access the content the given reference is pointing to.
+The validity of the reference is checked by @{const_typ readable}.
+Moreover, {\sc{Deref}} invalidates all descendant references to establish the uniqueness
+($kill\ t\ ts$).
+
+\begin{framed}
+\centering
+@{thm[mode=Rule] Deref} \sc{Deref}
+\end{framed}
+
+Last but not least, {\sc{Reborrow}} rule creates a new reference with a fresh tag reborrowing the given reference.
+The newly created reference is writable. Thus the original reference must be valid for writes.
+Reborrow is considered as the use of the original reference and hence it invalidates former children
+of the reference. As a result, the reborrow tree will have the original reference and the reborrowing
+reference as the last two element.
+
+\begin{framed}
+\sc{Reborrow} rule:
+\centering
+@{thm[mode=Rule] Reborrow}
+\end{framed}
 \<close>
 
-lemma box__writable: "(\<Gamma>, H, R, Box e) \<Down> (H', R', Reference p t) \<Longrightarrow> writable p t R'"
+(* proof automation *)
+(*<*)
+lemmas exp_sem_cases = exp_sem.cases[split_format(complete)] \<^marker>\<open>tag invisible\<close>
+lemmas exp_sem_induct = exp_sem.induct[split_format(complete)] \<^marker>\<open>tag invisible\<close>
+declare exp_sem.intros[simp, intro] \<^marker>\<open>tag invisible\<close>
+
+inductive_cases ConstE[elim!]: "(\<Gamma>, H, Const v) \<Down> v'" \<^marker>\<open>tag invisible\<close>
+inductive_cases VarE[elim!]: "(\<Gamma>, H, Var x) \<Down> v" \<^marker>\<open>tag invisible\<close>
+inductive_cases BoxE[elim!]: "(\<Gamma>, H, Box e) \<Down> v" \<^marker>\<open>tag invisible\<close>
+inductive_cases ReborrowE[elim!]: "(\<Gamma>, H, Reborrow e) \<Down> v" \<^marker>\<open>tag invisible\<close>
+inductive_cases DerefE[elim!]: "(\<Gamma>, H, Deref e) \<Down> v" \<^marker>\<open>tag invisible\<close>
+inductive_cases AlithE[elim!]: \<^marker>\<open>tag invisible\<close>
+  "(\<Gamma>, H, Plus e1 e2) \<Down> v"
+  "(\<Gamma>, H, Less e1 e2) \<Down> v"
+  "(\<Gamma>, H, Not e) \<Down> v"
+  "(\<Gamma>, H, And e1 e2) \<Down> v"
+
+(*>*)
+
+lemma reborrow_det_lemma: \<^marker>\<open>tag invisible\<close>
+  assumes
+    reborrow: "(\<Gamma>, H, Reborrow e) \<Down> E''" and
+    memory: "(v, ts) = H' ! p" and
+    readable: "readable p t H'" and
+    fresh_tag: "t' = fresh_tag H'" and
+    IH: "\<And>E'. (\<Gamma>, H, e) \<Down> E' \<Longrightarrow> E' = (H', Reference p t)"
+  shows "E'' = (H'[p := (v, kill t ts @ [t'])], Reference p t')"
+proof (rule ReborrowE[where \<Gamma> = \<Gamma> and H = H and v = E'' and e = e]) \<^marker>\<open>tag invisible\<close>
+  show "(\<Gamma>, H, Reborrow e) \<Down> E''" using reborrow by auto
+next
+  fix H'a pa ta va tsa
+  let ?fix_type = "fresh_tag H'a" (* without this line, the following let fails *)
+  let ?t'a = "Suc (fold max (fold (\<lambda>e ts. ts @ snd e) H'a []) 0)"
+  assume
+    e'': "E'' = (H'a[pa := (va, kill ta tsa @ [?t'a])], Reference pa ?t'a)" and
+    loc: "(\<Gamma>, H, e) \<Down>  (H'a, Reference pa ta)" and
+    memorya: "(va, tsa) = H'a ! pa" and
+    allocateda: "pa < length H'a" and
+    valida: "ta \<in> set (snd (H'a ! pa))"
+  moreover have "H'a = H'" "pa = p" "ta = t" using loc IH by auto
+  moreover have "(va, tsa) = (v, ts)" using calculation memory memorya by auto
+  moreover have "va = v" using calculation(9) by auto
+  moreover have "tsa = ts" using calculation(9) by auto
+  moreover have "?t'a = t'" using calculation(6) fresh_tag by auto
+  ultimately show "E'' = (H'[p := (v, kill t ts @ [t'])], Reference p t')" by auto
+qed
+
+text \<open>We can prove that the semantics of expressions is deterministic.\<close>
+
+lemma exp_sem_deterministic: "E \<Down> E' \<Longrightarrow> E \<Down> E'' \<Longrightarrow> E'' = E'"
+proof (induction E E' arbitrary: E'' rule: exp_sem.induct)
+  case (Reborrow \<Gamma> H e H' p t v ts t')
+  show ?case
+    using Reborrow.IH Reborrow.hyps(2) Reborrow.hyps(3) Reborrow.hyps(4)
+          Reborrow.prems readable_def reborrow_det_lemma by auto
+next
+  case (Deref \<Gamma> H e H' p t v ts)
+  then show ?case
+    by (smt DerefE Pair_inject val.inject(3))
+qed auto
+
+text \<open>The following lemmas are a sanity check of the semantics.
+We must be able to write through the references retrieved by {\sc{Box}} and {\sc{Reborrow}}\<close>
+
+lemma box__writable: "(\<Gamma>, H, Box e) \<Down> (H', Reference p t) \<Longrightarrow> writable p t H'"
   by auto
 
-lemma reborrow__writable: "(\<Gamma>, H, R, Reborrow e) \<Down> (H', R', Reference p t) \<Longrightarrow> writable p t R'"
+lemma reborrow__writable: "(\<Gamma>, H, Reborrow e) \<Down> (H', Reference p t) \<Longrightarrow> writable p t H'"
   by auto
 
-code_pred exp_sem .
+code_pred [show_modes] exp_sem .
 
 end
