Unique.thy
@@ -2,43 +2,63 @@ theory Unique
   imports Main Definitions Exp Star
 begin
 
-section \<open>Semantics\<close>
+section \<open>Semantics of Commands\<close>
 
-type_synonym config = "gamma * heap * reborrow * com"
+text \<open>This section describes the small-step semantics of commands.
+The configuration of an execution consists of
+\begin{itemize}
+  \item the variable environment $\Gamma$ (of type @{type gamma});
+  \item the heap $H$ (of type @{type heap}) which holds the actual data and the reborrow trees
+  for each address; and
+  \item the command to be executed $c$ (of type @{type com}).
+\end{itemize}\<close>
+
+type_synonym config = "gamma * heap * com"
 inductive com_sem :: "config \<Rightarrow> config \<Rightarrow> bool" (infix "\<rightarrow>" 65)
 where
-  VAssign: "(\<Gamma>, H, R, e) \<Down> (H', R', v)
-            \<Longrightarrow> (\<Gamma>, H, R, x ::= e) \<rightarrow> (\<Gamma>(x := Some v), H', R', Skip)" |
-  (* TODO: check validity of pointer? *)
-  HAssign: "\<lbrakk>(\<Gamma>, H, R, e\<^sub>l) \<Down> (H', R', Reference p t);
-             (\<Gamma>, H', R', e\<^sub>v) \<Down> (H'', R'', v);
-             writable p t R''\<rbrakk>
-            \<Longrightarrow> (\<Gamma>, H, R, *e\<^sub>l ::= e\<^sub>v) \<rightarrow> (\<Gamma>, H''(p := Some v), R''(p \<mapsto> kill t (the (R'' p))), Skip)" |
-  SeqL: "(\<Gamma>, H, R, Skip;; c) \<rightarrow> (\<Gamma>, H, R, c)" |
-  SeqR: "(\<Gamma>, H, R, C1) \<rightarrow> (\<Gamma>', H', R', c') \<Longrightarrow> (\<Gamma>, H, R, c1;; c2) \<rightarrow> (\<Gamma>', H', R', c';; c2)" |
-  IfTrue: "(\<Gamma>, H, R, b) \<Down> (H', R', VBool True)
-           \<Longrightarrow> (\<Gamma>, H, R, IF b THEN c1 ELSE c2) \<rightarrow> (\<Gamma>, H', R', c1)" |
-  IfFlase: "(\<Gamma>, H, R, b) \<Down> (H', R', VBool False)
-           \<Longrightarrow> (\<Gamma>, H, R, IF b THEN c1 ELSE c2) \<rightarrow> (\<Gamma>, H', R', c2)" |
-  While: "(\<Gamma>, H, R, WHILE b DO c) \<rightarrow> (\<Gamma>, H, R, IF b THEN (c;; WHILE b DO c) ELSE Skip)"
+  VAssign: "(\<Gamma>, H, e) \<Down> (H', v)
+            \<Longrightarrow> (\<Gamma>, H, x ::= e) \<rightarrow> (\<Gamma>(x \<mapsto> v), H', Skip)" |
+  HAssign: "\<lbrakk>(\<Gamma>, H, e\<^sub>l) \<Down> (H', Reference p t);
+             (\<Gamma>, H', e\<^sub>v) \<Down> (H'', v);
+             writable p t H''\<rbrakk>
+            \<Longrightarrow> (\<Gamma>, H, *e\<^sub>l ::= e\<^sub>v) \<rightarrow> (\<Gamma>, H''[p := (v, kill t (snd (H'' ! p)))], Skip)" |
+  SeqL: "(\<Gamma>, H, Skip;; c) \<rightarrow> (\<Gamma>, H, c)" |
+  SeqR: "(\<Gamma>, H, c1) \<rightarrow> (\<Gamma>', H', c') \<Longrightarrow> (\<Gamma>, H, c1;; c2) \<rightarrow> (\<Gamma>', H', c';; c2)" |
+  IfTrue: "(\<Gamma>, H, b) \<Down> (H', VBool True)
+           \<Longrightarrow> (\<Gamma>, H, IF b THEN c1 ELSE c2) \<rightarrow> (\<Gamma>, H', c1)" |
+  IfFlase: "(\<Gamma>, H, b) \<Down> (H', VBool False)
+           \<Longrightarrow> (\<Gamma>, H, IF b THEN c1 ELSE c2) \<rightarrow> (\<Gamma>, H', c2)" |
+  While: "(\<Gamma>, H, WHILE b DO c) \<rightarrow> (\<Gamma>, H, IF b THEN (c;; WHILE b DO c) ELSE Skip)"
+
+code_pred [show_modes] com_sem .
+
+lemmas com_sem_cases = com_sem.cases[split_format(complete)] \<^marker>\<open>tag invisible\<close>
+lemmas com_sem_induct = com_sem.induct[split_format(complete)] \<^marker>\<open>tag invisible\<close>
+
+declare com_sem.intros[simp, intro] \<^marker>\<open>tag invisible\<close>
 
 (* We declare safe elimination rules (automatically applied I guess?) *)
-inductive_cases [elim!]:
-  "(\<Gamma>, H, R, x ::= e) \<rightarrow> cfg"
-  "(\<Gamma>, H, R, *e\<^sub>l ::= e\<^sub>v) \<rightarrow> cfg"
-  "(\<Gamma>, H, R, Skip;; c) \<rightarrow> cfg"
-  "(\<Gamma>, H, R, c1;; c2) \<rightarrow> cfg"
-  "(\<Gamma>, H, R, IF b THEN c1 ELSE c2) \<rightarrow> cfg"
+inductive_cases ComE[elim!]: \<^marker>\<open>tag invisible\<close>
+  "(\<Gamma>, H, x ::= e) \<rightarrow> cfg"
+  "(\<Gamma>, H, *e\<^sub>l ::= e\<^sub>v) \<rightarrow> cfg"
+  "(\<Gamma>, H, Skip;; c) \<rightarrow> cfg"
+  "(\<Gamma>, H, c1;; c2) \<rightarrow> cfg"
+  "(\<Gamma>, H, IF b THEN c1 ELSE c2) \<rightarrow> cfg"
 
 (* WHILE might not terminate, so we declare it as an unsafe elimination rule *)
-inductive_cases WhileE[elim]: "(\<Gamma>, H, R, WHILE b DO c) \<rightarrow> cfg"
-thm WhileE
+inductive_cases WhileE[elim]: "(\<Gamma>, H, WHILE b DO c) \<rightarrow> cfg" \<^marker>\<open>tag invisible\<close>
 
 abbreviation com_sem_steps :: "config \<Rightarrow> config \<Rightarrow> bool" (infix "\<rightarrow>\<^sup>*" 65) where
   "cfg \<rightarrow>\<^sup>* cfg' == star com_sem cfg cfg'"
 
 text \<open>
-  Figure \ref{fig:com} shows the assignment rules. Other commands are standard.
+Figure \ref{fig:com} shows the assignment rules. Other commands are standard.
+
+The {\sc{VAssign}} rule assigns a value to the variable while
+the {\sc{HAssign}} rule to the location the reference on the left hand side is referring to.
+To assign through a reference, the reference must be valid for writes.
+Moreover, the write is considered as a use of the reference; it will invalidate the child references.
+
 \begin{figure}[h]
 \centering
 \begin{framed}
@@ -50,56 +70,163 @@ text \<open>
 \end{figure}
 \<close>
 
-code_pred com_sem .
+text \<open>The following lemmas show that the execution of the commands is deterministic.\<close>
 
-section \<open>Choosing fresh addresses/tags deterministically\<close>
+definition final :: "config \<Rightarrow> bool" where
+  "final cfg \<longleftrightarrow> (case cfg of (_, _, Skip) \<Rightarrow> True | _ \<Rightarrow> False)"
 
-definition empty :: "'a \<Rightarrow> 'b option" where
-  "empty = (\<lambda>_. None)"
+definition stuck :: "config \<Rightarrow> bool" where
+  "stuck cfg \<longleftrightarrow> (case cfg of
+     (_, _, Skip) \<Rightarrow> False |
+     _ \<Rightarrow> \<not>(\<exists>cfg'. cfg \<rightarrow> cfg'))"
 
-inductive packed_heap :: "nat \<Rightarrow> heap \<Rightarrow> bool" where
-  EmptyH: "packed_heap 0 empty" |
-  NextH: "packed_heap n H \<Longrightarrow> packed_heap (n + 1) (H(Address n \<mapsto> v))"
+lemma skip_final_noteq[simp]: "(\<Gamma>, H, c) \<rightarrow> (\<Gamma>', H', c') \<Longrightarrow> c \<noteq> Skip"
+proof (cases rule: com_sem_cases)
+qed auto
 
-lemma packed_heap__domain: "packed_heap n H \<Longrightarrow> (\<forall>n'. n' \<ge> n \<longleftrightarrow> H (Address n') = None)"
-proof (induction rule: packed_heap.induct)
-  case EmptyH
-  then show ?case
-    by (simp add: Unique.empty_def)
-next
-  case (NextH n H v)
-  then show ?case
-    by (metis One_nat_def add.right_neutral add_Suc_right address.inject
-        fun_upd_apply le_less le_simps(3) not_le option.discI)
+lemma skip_final[simp]: "\<not>(\<Gamma>, H, Skip) \<rightarrow> (\<Gamma>', H', c)"
+proof
+  assume "(\<Gamma>, H, Skip) \<rightarrow> (\<Gamma>', H', c)"
+  thus False using skip_final_noteq by blast
 qed
 
-lemma packed_heap__fresh: "packed_heap n H \<Longrightarrow> fresh (Address n) H"
-proof (induction rule: packed_heap.induct)
-  case EmptyH
+lemma com_sem_deterministic: "cfg \<rightarrow> cfg' \<Longrightarrow> cfg \<rightarrow> cfg'' \<Longrightarrow> cfg'' = cfg'"
+proof (induction arbitrary: cfg'' rule: com_sem.induct)
+  case (VAssign \<Gamma> H e H' v x)
   then show ?case
-    by (simp add: Unique.empty_def fresh_def)
+    using exp_sem_deterministic by auto
 next
-  case (NextH n H v)
+  case (HAssign \<Gamma> H e\<^sub>l H' p t e\<^sub>v H'' v)
   then show ?case
-    by (meson fresh_def le_less packed_heap.NextH packed_heap__domain)
+    by (smt ComE(2) Pair_inject exp_sem_deterministic val.inject(3))
+next
+  case (SeqL \<Gamma> H c)
+  then show ?case using skip_final by auto
+next
+  case (SeqR \<Gamma> H c1 \<Gamma>' H' c' c2)
+  then show ?case by (metis ComE(4) prod.inject skip_final)
+next
+  case (IfTrue \<Gamma> H b H' c1 c2)
+then show ?case using exp_sem_deterministic by fastforce
+next
+  case (IfFlase \<Gamma> H b H' c1 c2)
+then show ?case using exp_sem_deterministic by fastforce
+next
+  case (While \<Gamma> H b c)
+  then show ?case by auto
 qed
 
-definition packed_tags :: "nat \<Rightarrow> reborrow \<Rightarrow> bool" where
-  "packed_tags n R \<longleftrightarrow> tags R = {Tag k | k. k < n}"
+lemmas star_induct' = star.induct[of "(\<rightarrow>)", split_format(complete)] \<^marker>\<open>tag invisible\<close>
 
-lemma packed_tags__fresh: "packed_tags n R \<Longrightarrow> fresh_tag (Tag n) R"
-  by (simp add: fresh_tag_def packed_tags_def)
+text \<open>We show the transitivity of @{const com_sem_steps}.\<close>
+
+lemma com_seql_trans:
+  "(\<Gamma>, H, c1) \<rightarrow>\<^sup>* (\<Gamma>', H', c1') \<Longrightarrow> (\<Gamma>, H, c1;; c2) \<rightarrow>\<^sup>* (\<Gamma>', H', c1';; c2)"
+proof (induction rule: star_induct')
+  case (refl a a b)
+  then show ?case by simp
+next
+  case (step a a b a a b a a b)
+  then show ?case by (meson SeqR star.simps)
+qed
 
 section \<open>Code examples\<close>
 
-text \<open>The following code accesss \<close>
+subsection \<open>Invalidating a reference\<close>
 
-definition XYX :: com where
-  "XYX = 
+text \<open>Consider the following Rust program.
+\begin{minted}[linenos]{rust}
+let mut root = Box::new(42);
+let mut px = &mut *root; // reborrowing from root
+*px = 100;
+let mut py = &mut *root; // another reborrow. invalidates px
+*py = 200;
+// *px = 300 // this write is invalid.
+\end{minted}
+
+In line 1, we create a box that contains 42 in the heap.
+In the following two lines, we reborrow from it and use the reference to write.
+The interesting part is line 4. In this line, we create a new reference from \rust{root}.
+As this reborrow asserts that \rust{py} is the unique reference to the box,
+\rust{px} must be invalidated at this point.
+Therefore, if we remove the comment in line 6, the program will perform an invalid write
+(thus rustc will reject the program).
+
+Let's execute the program with Unique.
+The following command is the translation of the program above without the last commented line.\<close>
+
+definition XY :: com where
+  "XY =
     ''root'' ::= Box (Const (VInt 42));;
     ''px'' ::= Reborrow (Var ''root'');;
     *(Var ''px'') ::= Const (VInt 100);;
     ''py'' ::= Reborrow (Var ''root'');;
-    *(Var ''px'') ::= Const (VInt 200)"
+    *(Var ''py'') ::= Const (VInt 200)"
+
+text \<open>We can let Isabelle compute the program.\<close>
+
+values "{(map \<Gamma> [''root'', ''px'', ''py''], H, c) |
+         \<Gamma> H c. (Map.empty, [], XY) \<rightarrow>\<^sup>* (\<Gamma>, H, c)}"
+
+text \<open>The following shows the variable environment and the heap at the end of execution.\<close>
+
+abbreviation \<Gamma>\<^sub>X\<^sub>Y :: gamma where
+  "\<Gamma>\<^sub>X\<^sub>Y == [''root'' \<mapsto> Reference 0 1, ''px'' \<mapsto> Reference 0 2, ''py'' \<mapsto> Reference 0 3]"
+abbreviation H\<^sub>X\<^sub>Y :: heap where
+  "H\<^sub>X\<^sub>Y == [(VInt 200, [1, 3])]"
+
+text \<open>We can also prove that the program result in the state shown above in theory,
+but it's really tedious (why can't Isabelle prove it by computing the execution?).
+The actual proof is left to the reader.\<close>
+
+lemma final_xy: "(Map.empty, [], XY) \<rightarrow>\<^sup>* (\<Gamma>\<^sub>X\<^sub>Y, H\<^sub>X\<^sub>Y, Skip)"
+  sorry \<^marker>\<open>tag important\<close>
+
+text \<open>We show that accessing through \rust{px} after the program will stuck.\<close>
+
+lemma intermediate_xyx: "(Map.empty, [], XY;; *(Var ''px'') ::= Const (VInt 300)) \<rightarrow>\<^sup>*
+  (\<Gamma>\<^sub>X\<^sub>Y, H\<^sub>X\<^sub>Y, *(Var ''px'') ::= Const (VInt 300))"
+  apply (rule star_trans)
+   prefer 2
+   apply (rule star_step1)
+   apply (rule SeqL)
+  apply (rule com_seql_trans)
+  apply (rule final_xy)
+  done
+
+lemma stuck_xyx: "stuck
+   (\<Gamma>\<^sub>X\<^sub>Y, H\<^sub>X\<^sub>Y, *(Var ''px'') ::= Const (VInt 300))"
+  apply (simp add: stuck_def)
+  apply (rule allI)+
+  apply (rule notI)
+  apply (rule ComE(1))
+   apply (auto)
+  done
+
+lemma "\<exists>cfg. (Map.empty, [], XY;; *(Var ''px'') ::= Const (VInt 300)) \<rightarrow>\<^sup>* cfg
+           \<and> stuck cfg"
+  apply (rule exI)
+  apply (rule conjI)
+   apply (rule intermediate_xyx)
+  apply (rule stuck_xyx)
+  done
+
+subsection \<open>Swap\<close>
+
+text \<open>The following program swaps the content the given two references pointing to.\<close>
+
+fun swap :: "exp \<Rightarrow> exp \<Rightarrow> com" where
+  "swap x y =
+    ''reborrow_x'' ::= Reborrow x;;
+    ''reborrow_y'' ::= Reborrow y;;
+    ''tmp'' ::= Deref (Var ''reborrow_x'');;
+    *(Var ''reborrow_x'') ::= Deref (Var ''reborrow_y'');;
+    *(Var ''reborrow_y'') ::= Var ''tmp''"
+
+text \<open>We can see the content swapped during the execution by running it on Isabelle.\<close>
+
+values "{H | \<Gamma> H c. (Map.empty, [], swap (Box (Const (VInt 42))) (Box (Const (VInt 100)))) \<rightarrow>\<^sup>* (\<Gamma>, H, c)}"
+
+text \<open>Proving the correctness of @{const swap} would need a Hoare Logic. The road continues...\<close>
 
 end
