ROOT
@@ -1,7 +1,9 @@
 session "rust-verification" = HOL +
-  options [document = pdf, document_output = "output"]
-  (*theories [document = false]*)
+  options [document = pdf, document_output = "output", document_variants="document=/proof", quick_and_dirty]
+  sessions
+    "HOL-Library" (* for HOL-Library.LaTeXsugar *)
   theories [show_question_marks = false]
     Unique
   document_files
     "root.tex"
+    "root.bib"
